Source/Concurrency/LinearPermissionInstrumentation.cs
@@ -7,22 +7,19 @@ namespace Microsoft.Boogie
   public class LinearPermissionInstrumentation
   {
     private CivlTypeChecker civlTypeChecker;
-    private LinearTypeChecker linearTypeChecker;
     private int layerNum;
-    private Dictionary<Absy, Absy> absyMap;
+    private AbsyMap absyMap;
     private Dictionary<string, Variable> domainNameToHoleVar;
     private Dictionary<Variable, Variable> localVarMap;
 
     public LinearPermissionInstrumentation(
       CivlTypeChecker civlTypeChecker,
-      LinearTypeChecker linearTypeChecker,
       int layerNum,
-      Dictionary<Absy, Absy> absyMap,
+      AbsyMap absyMap,
       Dictionary<string, Variable> domainNameToHoleVar,
       Dictionary<Variable, Variable> localVarMap)
     {
       this.civlTypeChecker = civlTypeChecker;
-      this.linearTypeChecker = linearTypeChecker;
       this.layerNum = layerNum;
       this.absyMap = absyMap;
       this.domainNameToHoleVar = domainNameToHoleVar;
@@ -31,12 +28,10 @@ namespace Microsoft.Boogie
 
     public LinearPermissionInstrumentation(
       CivlTypeChecker civlTypeChecker,
-      LinearTypeChecker linearTypeChecker,
       int layerNum,
-      Dictionary<Absy, Absy> absyMap)
+      AbsyMap absyMap)
     {
       this.civlTypeChecker = civlTypeChecker;
-      this.linearTypeChecker = linearTypeChecker;
       this.layerNum = layerNum;
       this.absyMap = absyMap;
       this.domainNameToHoleVar = new Dictionary<string, Variable>();
@@ -65,6 +60,7 @@ namespace Microsoft.Boogie
 
     public Dictionary<string, Expr> PermissionExprs(Absy absy)
     {
+      var linearTypeChecker = civlTypeChecker.linearTypeChecker;
       var domainNameToScope = new Dictionary<string, HashSet<Variable>>();
       foreach (var domainName in linearTypeChecker.linearDomains.Keys)
       {
@@ -128,6 +124,7 @@ namespace Microsoft.Boogie
 
     private List<Expr> DisjointnessExprs(IEnumerable<Variable> availableVars)
     {
+      var linearTypeChecker = civlTypeChecker.linearTypeChecker;
       var domainNameToScope = new Dictionary<string, HashSet<Variable>>();
       foreach (var domainName in linearTypeChecker.linearDomains.Keys)
       {
@@ -164,15 +161,15 @@ namespace Microsoft.Boogie
     {
       if (absy is Implementation impl)
       {
-        return FilterInParams((MapAbsy(impl) as Implementation).InParams);
+        return FilterInParams(absyMap.OriginalOrInput(impl).InParams);
       }
 
       if (absy is Procedure proc)
       {
-        return FilterInParams((MapAbsy(proc) as Procedure).InParams);
+        return FilterInParams(absyMap.OriginalOrInput(proc).InParams);
       }
 
-      return linearTypeChecker.AvailableLinearVars(MapAbsy(absy)).Where(v =>
+      return civlTypeChecker.linearTypeChecker.AvailableLinearVars(absyMap[absy]).Where(v =>
         !(v is GlobalVariable) &&
         civlTypeChecker.LocalVariableLayerRange(v).Contains(layerNum));
     }
@@ -190,12 +187,13 @@ namespace Microsoft.Boogie
     private IEnumerable<Variable> Filter(IEnumerable<Variable> locals, Predicate<LinearKind> pred)
     {
       return locals.Where(v =>
-        pred(linearTypeChecker.FindLinearKind(v)) &&
+        pred(civlTypeChecker.linearTypeChecker.FindLinearKind(v)) &&
         civlTypeChecker.LocalVariableLayerRange(v).Contains(layerNum));
     }
 
     private IEnumerable<Variable> LinearGlobalVars()
     {
+      var linearTypeChecker = civlTypeChecker.linearTypeChecker;
       return linearTypeChecker.program.GlobalVariables.Where(v =>
         linearTypeChecker.FindLinearKind(v) == LinearKind.LINEAR &&
         civlTypeChecker.GlobalVariableLayerRange(v).Contains(layerNum));
@@ -204,11 +202,6 @@ namespace Microsoft.Boogie
     private Variable MapVariable(Variable v)
     {
       return localVarMap.ContainsKey(v) ? localVarMap[v] : v;
-    }
-
-    private Absy MapAbsy(Absy absy)
-    {
-      return absyMap.ContainsKey(absy) ? absyMap[absy] : absy;
     }
   }
 }
